Gt3/HasTy/Subst.lean
@@ -85,3 +85,112 @@ theorem Ctx.HasTy.ls_clamped {K : Finset String} {Γ σ Δ} (hσ : S1 Γ σ Δ) 
       <;> apply_assumption
       <;> assumption
     }
+
+theorem Ctx.S1.castEqOn {Γ σ σ' Δ}
+  (hστ : S1 Γ σ Δ) (hσ : σ.EqOn Δ.dv σ')
+  : S1 Γ σ' Δ := by
+  induction hστ with
+  | nil => constructor; assumption
+  | cons' _ _ _ hΔA =>
+    have hΔA' := Finset.Subset.trans hΔA.scoped (Finset.subset_insert ?x _)
+    (constructor <;> first
+    | assumption
+    | apply_assumption ; apply Tm.VSubst.EqOn.anti _ ‹_›
+    | repeat first
+      | rw [<-Tm.ls_eqOn_sub_fvs (h := hσ)]
+      | rw [<-Tm.ls_eqOn_sub_fvs (h := hτ)]
+      | rw [<-hσ.get _ Ctx.head_mem_dv]
+      | rw [<-hτ.get _ Ctx.head_mem_dv]
+      | assumption
+    ) ; simp
+
+theorem Ctx.S1.clamp {Γ σ Δ} (hσ : S1 Γ σ Δ) : S1 Γ (σ.clamp Δ.dv) Δ
+  := hσ.castEqOn (σ.clamp_eqOn Δ.dv).symm
+
+theorem Ctx.S1.unclamp {Γ σ Δ}
+  (hσ : S1 Γ (σ.clamp Δ.dv) Δ)
+  : S1 Γ σ Δ
+  := hσ.castEqOn (σ.clamp_eqOn Δ.dv)
+
+theorem Ctx.HasTy.ls {Γ σ Δ} (hσ : S1 Γ σ Δ) {A a} (h : HasTy Δ A a)
+  : HasTy Γ (σ • A) (σ • a) := by
+  convert (h.ls_clamped hσ.clamp (Tm.VSubst.clamped _ _)) using 1 <;>
+  rw [Tm.ls_clamp_sub_fvs] <;>
+  simp only [h.scoped_all]
+
+theorem Ctx.S1.clamp_iff {Γ σ Δ}
+  : S1 Γ (σ.clamp Δ.dv) Δ ↔ S1 Γ σ Δ
+  := ⟨unclamp, clamp⟩
+
+def Ctx.PSEq' (Γ Δ : Ctx) : Prop := S1 Γ 1 Δ
+
+def Ctx.PSEq'.refl {Γ Δ} (h : PSEq' Γ Δ) : PSEq Γ Δ := S1.refl h
+
+theorem Ctx.S1.one {Γ} (hΓ : Ok Γ) : S1 Γ 1 Γ := by
+  induction hΓ with
+  | nil => constructor; constructor
+  | cons hΓ hx hA =>
+    have hA' := hA.wk0 hx hA
+    have hΓxA := hΓ.cons hx hA
+    constructor <;> first | simp [HasTy.top_var_iff, *] | apply S1.wk0 <;> assumption
+
+theorem Ctx.S1.rename_top' {Γ x y A B} (hx : x ∉ Γ.dv) (hy : y ∉ Γ.dv) (hAB : TyEq Γ A B)
+  : S1 (Γ.cons x A) (.lset (.fv x) y) (Γ.cons y B) :=
+  have hABt := hAB.top_var hx;
+  have hxA := hAB.lhs.wk0 hx hAB.lhs
+  have hxB := hAB.rhs.wk0 hx hAB.lhs
+  have hAy := Finset.not_mem_subset hAB.lhs.scoped hy;
+  have hBy := Finset.not_mem_subset hAB.rhs.scoped hy;
+  have hAy' := Tm.ls_lset_not_mem (hx := hAy)
+  have hBy' := Tm.ls_lset_not_mem (hx := hBy)
+  by
+    apply S1.cons' (.wk0
+      ((S1.one hAB.ok).castEqOn
+        (fun z hz => by simp [Tm.get_lset]; intro h; cases h; contradiction)
+      ) hx hAB.lhs)
+    <;> simp [hAB.rhs, *]
+
+theorem Ctx.S1.rename_top {Γ x y A} (hx : x ∉ Γ.dv) (hy : y ∉ Γ.dv) (hA : IsTy Γ A)
+  : S1 (Γ.cons x A) (.lset (.fv x) y) (Γ.cons y A) := rename_top' hx hy hA
+
+theorem Ctx.HasTy.ps' {Γ Δ} (hσ : PSEq' Γ Δ) {A a} (h : HasTy Δ A a)
+  : HasTy Γ A a := by convert h.ls hσ <;> simp
+
+theorem Ctx.PSEq'.retype_top {Γ x A B} (hx : x ∉ Γ.dv) (hAB : TyEq Γ A B)
+  : PSEq' (Γ.cons x A) (Γ.cons x B)
+  := by convert (S1.rename_top' hx hx hAB) using 0; simp [Ctx.PSEq']
+
+theorem Ctx.HasTy.cast_top {Γ x A B C a} (hAB : TyEq Γ A B) (h : HasTy (Γ.cons x B) C a)
+  : HasTy (Γ.cons x A) C a := h.ps' (.retype_top h.ok.var hAB)
+
+theorem Ctx.HasTy.cast_top' {Γ x ℓ A B C a} (hAB : JEq Γ (.univ ℓ) A B) (h : HasTy (Γ.cons x B) C a)
+  : HasTy (Γ.cons x A) C a := h.cast_top hAB.ty_eq
+
+-- theorem Ctx.HasTy.sjeq_clamped {K : Finset String} {Γ σ τ Δ} (hσ : SEq Γ σ τ Δ) {A a}
+--   (h : HasTy Δ A a) (hK : σ.Clamped K)
+--   : SJEq Γ σ τ A a := by induction h generalizing Γ with
+--   | fv _ hx => exact hx.sjeq hσ
+--   | cast_level =>
+--     simp only [Ctx.SJEq, forall_and] at *
+--     try casesm* _ ∧ _
+--     constructor <;> apply JEq.cast_level <;> apply_assumption <;> assumption
+--   | cast => stop apply cast <;> (first | apply_assumption | apply TyEq.ls1) <;> assumption
+--   | _ =>
+--     stop
+--     constructor <;>
+--     first
+--     | (try simp only [<-Tm.smul_def, <-Tm.ls_lst])
+--       ; (first | apply_assumption | apply TyEq.ls1)
+--       <;> assumption
+--     | exact hσ.src_ok
+--     | {
+--       intro x hx
+--       rename Finset String => L
+--       have ⟨hxK, hxL, hxΓ, hxΔ⟩ : x ∉ K ∧ x ∉ L ∧ x ∉ hσ.src.dv ∧ x ∉ hσ.trg.dv
+--         := by simp only [<-Finset.notMem_union]; exact hx
+--       simp only [<-Tm.smul_def, Tm.open_ls_clamped (hv := hK) (hx := hxK)]
+--       apply_assumption
+--       <;> first | assumption | apply S1.lift_clamped
+--       <;> apply_assumption
+--       <;> assumption
+--     }
