Gt3/HasTy/Cmp.lean
@@ -1,0 +1,43 @@
+import Gt3.HasTy.Subst
+
+def Ctx.Cmp (Γ : Ctx) (A a b : Tm 0) : Prop := HasTy Γ A a ∧ HasTy Γ A b
+
+theorem Ctx.Cmp.cast_level {Γ ℓ A B} (h : Cmp Γ (.univ ℓ) A B) : Cmp Γ (.univ (ℓ + 1)) A B
+  := ⟨h.left.cast_level, h.right.cast_level⟩
+
+theorem Ctx.Cmp.cast' {Γ ℓ A A' a b} (hA : JEq Γ (.univ ℓ) A A') (hab : Cmp Γ A a b)
+  : Cmp Γ A' a b := ⟨hab.left.cast' hA, hab.right.cast' hA⟩
+
+theorem Ctx.Cmp.symm {Γ A a b} (h : Cmp Γ A a b) : Cmp Γ A b a
+  := ⟨h.right, h.left⟩
+
+theorem Ctx.Cmp.trans {Γ A a b c} (h : Cmp Γ A a b) (h' : Cmp Γ A b c) : Cmp Γ A a c
+  := ⟨h.left, h'.right⟩
+
+-- theorem Ctx.JEq.cmp {Γ A a b} (h : JEq Γ A a b) : Cmp Γ A a b := by induction h with
+--   | nil_ok => sorry
+--   | cons_ok => sorry
+--   | cast_level => apply Cmp.cast_level; assumption
+--   | cast' => apply Cmp.cast' <;> assumption
+--   | symm => apply Cmp.symm; assumption
+--   | trans => apply Cmp.trans <;> assumption
+--   | pi =>
+--     sorry
+--   | abs =>
+--     sorry
+--   | app' => sorry
+--   | beta_app => sorry
+--   | _ =>
+--     simp only [Ctx.Cmp, forall_and] at *
+--     casesm* _ ∧ _
+--     apply And.intro <;>
+--     first
+--     | assumption
+--     | {
+--         constructor <;> first
+--         | assumption
+--         | apply Ctx.JEq.ok ; assumption
+--         | apply JEq.ty_eq ; assumption
+--         -- | intros <;> apply HasTy.cast_top' <;> fail
+--         -- | fail
+--       }
